examples/insertion_sort/insertion_sort_InsertionSortGen_WP_parameter_insertion_sort_1.v
@@ -80,50 +80,48 @@ Definition exchange {a:Type} {a_WT:WhyType a} (a1:(@array a a_WT))
   ((~ (k = i)) -> ((~ (k = j)) -> ((get a1 k) = (get a2 k)))))))).
 
 (* Why3 assumption *)
-Definition map_permut_sub {a:Type} {a_WT:WhyType a} (a1:(@array a a_WT))
-  (a2:(@array a a_WT)) (l:Z) (u:Z): Prop := ((length a1) = (length a2)) /\
+Definition permut {a:Type} {a_WT:WhyType a} (a1:(@array a a_WT)) (a2:(@array
+  a a_WT)) (l:Z) (u:Z): Prop := ((length a1) = (length a2)) /\
   (((0%Z <= l)%Z /\ (l <= (length a1))%Z) /\ (((0%Z <= u)%Z /\
-  (u <= (length a1))%Z) /\ (map.MapPermut.permut_sub (elts a1) (elts a2) l
-  u))).
+  (u <= (length a1))%Z) /\ (map.MapPermut.permut (elts a1) (elts a2) l u))).
 
 (* Why3 assumption *)
 Definition permut_sub {a:Type} {a_WT:WhyType a} (a1:(@array a a_WT))
-  (a2:(@array a a_WT)) (l:Z) (u:Z): Prop := ((length a1) = (length a2)) /\
-  (((0%Z <= l)%Z /\ (l <= (length a1))%Z) /\ (((0%Z <= u)%Z /\
-  (u <= (length a1))%Z) /\ ((map_eq_sub (elts a1) (elts a2) 0%Z l) /\
-  ((map.MapPermut.permut_sub (elts a1) (elts a2) l u) /\ (map_eq_sub
-  (elts a2) (elts a2) u (length a1)))))).
+  (a2:(@array a a_WT)) (l:Z) (u:Z): Prop := (map_eq_sub (elts a1) (elts a2)
+  0%Z l) /\ ((permut a1 a2 l u) /\ (map_eq_sub (elts a1) (elts a2) u
+  (length a1))).
 
 (* Why3 assumption *)
-Definition permut {a:Type} {a_WT:WhyType a} (a1:(@array a a_WT)) (a2:(@array
-  a a_WT)): Prop := ((length a1) = (length a2)) /\ (map.MapPermut.permut_sub
-  (elts a1) (elts a2) 0%Z (length a1)).
+Definition permut_all {a:Type} {a_WT:WhyType a} (a1:(@array a a_WT))
+  (a2:(@array a a_WT)): Prop := ((length a1) = (length a2)) /\
+  (map.MapPermut.permut (elts a1) (elts a2) 0%Z (length a1)).
 
-Axiom permut_refl : forall {a:Type} {a_WT:WhyType a}, forall (a1:(@array
-  a a_WT)), (permut a1 a1).
+Axiom permut_all_refl : forall {a:Type} {a_WT:WhyType a}, forall (a1:(@array
+  a a_WT)), (permut_all a1 a1).
 
-Axiom exchange_permut : forall {a:Type} {a_WT:WhyType a}, forall (a1:(@array
-  a a_WT)) (a2:(@array a a_WT)) (i:Z) (j:Z), (exchange a1 a2 i j) -> (permut
-  a1 a2).
+Axiom exchange_permut_all : forall {a:Type} {a_WT:WhyType a},
+  forall (a1:(@array a a_WT)) (a2:(@array a a_WT)) (i:Z) (j:Z), (exchange a1
+  a2 i j) -> (permut_all a1 a2).
 
-Axiom permut_sym : forall {a:Type} {a_WT:WhyType a}, forall (a1:(@array
-  a a_WT)) (a2:(@array a a_WT)), (permut a1 a2) -> (permut a2 a1).
+Axiom permut_all_sym : forall {a:Type} {a_WT:WhyType a}, forall (a1:(@array
+  a a_WT)) (a2:(@array a a_WT)), (permut_all a1 a2) -> (permut_all a2 a1).
 
-Axiom permut_trans : forall {a:Type} {a_WT:WhyType a}, forall (a1:(@array
-  a a_WT)) (a2:(@array a a_WT)) (a3:(@array a a_WT)), (permut a1 a2) ->
-  ((permut a2 a3) -> (permut a1 a3)).
+Axiom permut_all_trans : forall {a:Type} {a_WT:WhyType a}, forall (a1:(@array
+  a a_WT)) (a2:(@array a a_WT)) (a3:(@array a a_WT)), (permut_all a1 a2) ->
+  ((permut_all a2 a3) -> (permut_all a1 a3)).
 
-Axiom array_eq_permut : forall {a:Type} {a_WT:WhyType a}, forall (a1:(@array
-  a a_WT)) (a2:(@array a a_WT)), (array_eq a1 a2) -> (permut a1 a2).
+Axiom array_eq_permut_all : forall {a:Type} {a_WT:WhyType a},
+  forall (a1:(@array a a_WT)) (a2:(@array a a_WT)), (array_eq a1 a2) ->
+  (permut_all a1 a2).
 
 Axiom permut_sub_weakening : forall {a:Type} {a_WT:WhyType a},
   forall (a1:(@array a a_WT)) (a2:(@array a a_WT)) (l1:Z) (u1:Z) (l2:Z)
   (u2:Z), (permut_sub a1 a2 l1 u1) -> (((0%Z <= l2)%Z /\ (l2 <= l1)%Z) ->
   (((u1 <= u2)%Z /\ (u2 <= (length a1))%Z) -> (permut_sub a1 a2 l2 u2))).
 
-Axiom permut_sub_permut : forall {a:Type} {a_WT:WhyType a},
+Axiom permut_sub_permut_all : forall {a:Type} {a_WT:WhyType a},
   forall (a1:(@array a a_WT)) (a2:(@array a a_WT)) (l:Z) (u:Z), (permut_sub
-  a1 a2 l u) -> (permut a1 a2).
+  a1 a2 l u) -> (permut_all a1 a2).
 
 Axiom elt : Type.
 Parameter elt_WhyType : WhyType elt.
@@ -161,21 +159,22 @@ Theorem WP_parameter_insertion_sort : forall (a:Z) (a1:(@map.Map.map Z _
   elt elt_WhyType)), let a2 := (mk_array a a1) in ((0%Z <= a)%Z -> let o :=
   (a - 1%Z)%Z in ((1%Z <= o)%Z -> forall (a3:(@map.Map.map Z _
   elt elt_WhyType)), forall (i:Z), ((1%Z <= i)%Z /\ (i <= o)%Z) ->
-  (((sorted_sub a3 0%Z i) /\ (permut a2 (mk_array a a3))) ->
+  (((sorted_sub a3 0%Z i) /\ (permut_all a2 (mk_array a a3))) ->
   (((0%Z <= a)%Z /\ ((0%Z <= i)%Z /\ (i < a)%Z)) -> let v := (map.Map.get a3
   i) in forall (j:Z) (a4:(@map.Map.map Z _ elt elt_WhyType)),
-  (((0%Z <= j)%Z /\ (j <= i)%Z) /\ ((permut a2 (mk_array a (map.Map.set a4 j
-  v))) /\ ((forall (k1:Z) (k2:Z), ((0%Z <= k1)%Z /\ ((k1 <= k2)%Z /\
-  (k2 <= i)%Z)) -> ((~ (k1 = j)) -> ((~ (k2 = j)) -> (le (map.Map.get a4 k1)
-  (map.Map.get a4 k2))))) /\ forall (k:Z), (((j + 1%Z)%Z <= k)%Z /\
-  (k <= i)%Z) -> (le v (map.Map.get a4 k))))) -> ((0%Z < j)%Z -> let o1 :=
-  (j - 1%Z)%Z in (((0%Z <= a)%Z /\ ((0%Z <= o1)%Z /\ (o1 < a)%Z)) -> ((~ (le
-  (map.Map.get a4 o1) v)) -> let o2 := (j - 1%Z)%Z in (((0%Z <= o2)%Z /\
-  (o2 < a)%Z) -> (((0%Z <= j)%Z /\ (j < a)%Z) -> forall (a5:(@map.Map.map Z _
+  (((0%Z <= j)%Z /\ (j <= i)%Z) /\ ((permut_all a2 (mk_array a
+  (map.Map.set a4 j v))) /\ ((forall (k1:Z) (k2:Z), ((0%Z <= k1)%Z /\
+  ((k1 <= k2)%Z /\ (k2 <= i)%Z)) -> ((~ (k1 = j)) -> ((~ (k2 = j)) -> (le
+  (map.Map.get a4 k1) (map.Map.get a4 k2))))) /\ forall (k:Z),
+  (((j + 1%Z)%Z <= k)%Z /\ (k <= i)%Z) -> (le v (map.Map.get a4 k))))) ->
+  ((0%Z < j)%Z -> let o1 := (j - 1%Z)%Z in (((0%Z <= a)%Z /\
+  ((0%Z <= o1)%Z /\ (o1 < a)%Z)) -> ((~ (le (map.Map.get a4 o1) v)) ->
+  let o2 := (j - 1%Z)%Z in (((0%Z <= o2)%Z /\ (o2 < a)%Z) ->
+  (((0%Z <= j)%Z /\ (j < a)%Z) -> forall (a5:(@map.Map.map Z _
   elt elt_WhyType)), ((0%Z <= a)%Z /\ (a5 = (map.Map.set a4 j (map.Map.get a4
   o2)))) -> ((exchange (mk_array a (map.Map.set a4 j v)) (mk_array a
   (map.Map.set a5 (j - 1%Z)%Z v)) (j - 1%Z)%Z j) -> forall (j1:Z),
-  (j1 = (j - 1%Z)%Z) -> (permut a2 (mk_array a (map.Map.set a5 j1
+  (j1 = (j - 1%Z)%Z) -> (permut_all a2 (mk_array a (map.Map.set a5 j1
   v))))))))))))).
 (* Why3 intros a a1 a2 h1 o h2 a3 i (h3,h4) (h5,h6) (h7,(h8,h9)) v j a4
         ((h10,h11),(h12,(h13,h14))) h15 o1 (h16,(h17,h18)) h19 o2 (h20,h21)
@@ -183,7 +182,7 @@ Theorem WP_parameter_insertion_sort : forall (a:Z) (a1:(@map.Map.map Z _
 intros a a1 a2 h1 o h2 a3 i (h3,h4) (h5,h6) (h7,(h8,h9)) v j a4
         ((h10,h11),(h12,(h13,h14))) h15 o1 (h16,(h17,h18)) h19 o2 (h20,h21)
         (h22,h23) a5 (h24,h25) h26 j1 h27.
-unfold permut in *.
+unfold permut_all in *.
 simpl; split; auto.
 simpl in h12.
 destruct h12 as (h12a & h12b).
